MSet/MMapInterface.v
@@ -12,13 +12,12 @@
     as well as the improved finite set interfaces in MSet.
 *)
 
+
 Require Export Bool SetoidList RelationClasses Morphisms
  RelationPairs Equalities Orders OrdersFacts.
-
 Set Implicit Arguments.
 
 Unset Strict Implicit.
-
 
 Definition Cmp (elt:Type)(cmp:elt->elt->bool) e1 e2 := cmp e1 e2 = true.
 
@@ -29,120 +28,93 @@ End TypElt.
 
 Module Type HasWOps (Import T:TypElt).
 
-  Section Types.
+  Section Foo.
+  Variable  A : Type.
 
-    Variable  A : Type.
+  Parameter empty : t A.
+  (** The empty map. *)
 
-    Parameter empty : t A.
-    (** The empty map. *)
+  Parameter is_empty : t A -> bool.
+  (** Test whether a map is empty or not. *)
 
-    Parameter is_empty : t A -> bool.
-    (** Test whether a map is empty or not. *)
+  Parameter mem : key -> t A -> bool.
+  (** [mem k m] tests whether [k] belongs to the map [m]. *)
+ 
+  Parameter find : key -> t A -> option A.
 
-    Parameter add : key -> A -> t A -> t A.
-    (** [add k m] returns a map containing all elements of [m],
-        plus one mapping [k] to [v]. If [k] was already in [m], then its value
-        is replaced by [v]. *)
+  Parameter add : key -> A -> t A -> t A.
+  (** [add k m] returns a map containing all elements of [m],
+  plus one mapping [k] to [v]. If [k] was already in [m], then its value
+  is replaced by [v]. *)
 
-    Parameter find : key -> t A -> option A.
-    (** [find x m] returns the current binding of [x] in [m],
-	    or [None] if no such binding exists. *)
+  Parameter singleton : key -> A -> t A.
+  (** [singleton k v] returns the one-element map containing only the key [k]
+  that maps to [v]. *)
 
-    Parameter remove : key -> t A -> t A.
-    (** [remove k m] returns a map containing all elements of [m],
-        except [k]. If [k] was not in [m], [m] is returned unchanged. *)
+  Parameter remove : key -> t A -> t A.
+  (** [remove k m] returns a map containing all elements of [m],
+  except [k]. If [k] was not in [m], [m] is returned unchanged. *)
 
-    Parameter mem : key -> t A -> bool.
-    (** [mem k m] tests whether [k] belongs to the map [m]. *)
+  (*
+  TODO: Does not exist in FSet, OCaml has merge. What to do?
 
-    Variable A' A'' : Type.
+  Parameter union : t A -> t A -> t A.
+  (** Set union. *)
 
-    Parameter map : (A -> A') -> t A -> t A'.
-    (** [map f m] returns a map with same domain as [m], where the associated
-	    value a of all bindings of [m] has been replaced by the result of the
-	    application of [f] to [a]. Since Coq is purely functional, the order
-        in which the bindings are passed to [f] is irrelevant. *)
+  Parameter inter : t -> t -> t.
+  (** Set intersection. *)
 
-    Parameter mapi : (key -> A -> A') -> t A -> t A'.
-    (** Same as [map], but the function receives as arguments both the
-	    key and the associated value for each binding of the map. *)
+  Parameter diff : t -> t -> t.
+  (** Set difference. *)
+  *)
 
-    Parameter map2 :
-     (option A -> option A' -> option A'') -> t A -> t A' ->  t A''.
-    (** [map2 f m m'] creates a new map whose bindings belong to the ones
-        of either [m] or [m']. The presence and value for a key [k] is
-        determined by [f e e'] where [e] and [e'] are the (optional) bindings
-        of [k] in [m] and [m']. *)
+  Parameter equal : (A -> A -> bool) -> t A -> t A -> bool.
+  (** [equal val_eq m1 m2] tests whether the maps [m1] and [m2] are
+  equal, that is, contains the same keys, and values [v1] in [m1]
+  and [v2] in [m2] for a common key [k] must be equal according to
+  [val_eq]. *)
 
-    Parameter elements : t A -> list (key * A).
-    (** [elements m] returns an assoc list corresponding to the bindings
-        of [m], in any order. *)
+  Parameter subset : (A -> A -> bool) -> t A -> t A -> bool.
+  (** [subset val_eq m1 m2] tests whether the map [m1] is a subset of
+  the map [m2], where the values [v1] and [v2] for a common key [k]
+  must be equal according to [val_eq]. *)
 
-    Parameter cardinal : t A -> nat.
-    (** [cardinal m] returns the number of bindings in [m]. *)
+  Parameter fold : forall X : Type, (key -> A -> X -> X) -> t A -> X -> X.
+  (** [fold f m a] computes [(f kN vN ... (f k2 v2 (f k1 v1 a))...)],
+  where [k1 ... kN] are the keys, and [v1 ... vN] the corresponding values
+  of [m]. The order in which elements of [m] are presented to [f] is
+  unspecified. *)
 
-    Parameter fold : forall X : Type, (key -> A -> X -> X) -> t A -> X -> X.
-    (** [fold f m a] computes [(f kN vN ... (f k2 v2 (f k1 v1 a))...)],
-        where [k1 ... kN] are the keys, and [v1 ... vN] the corresponding values
-        of [m]. The order in which elements of [m] are presented to [f] is
-        unspecified. *)
+  Parameter for_all : (key -> A -> bool) -> t A -> bool.
+  (** [for_all p m] checks if all elements of the map [m]
+  satisfy the predicate [p]. *)
 
-    Parameter equal : (A -> A -> bool) -> t A -> t A -> bool.
-    (** [equal val_eq m1 m2] tests whether the maps [m1] and [m2] are
-        equal, that is, contains the same keys, and values [v1] in [m1]
-        and [v2] in [m2] for a common key [k] must be equal according to
-        [val_eq]. *)
+  Parameter exists_ : (key -> A -> bool) -> t A -> bool.
+  (** [exists p m] checks if at least one element of
+  the map [m] satisfies the predicate [p]. *)
 
-    (* TODO: This is the end of the original FMap.
-       * Is the rest really needed?
-       * If so, there probably are facts about it missing from MMapFacts, as
-         MMapFacts was based on the original FMap
-    *)
+  Parameter filter : (key -> A -> bool) -> t A -> t A.
+  (** [filter p m] returns the map of all elements in [m]
+  that satisfy predicate [p]. *)
 
-    Parameter singleton : key -> A -> t A.
-    (** [singleton k v] returns the one-element map containing only the key [k]
-        that maps to [v]. *)
+  Parameter partition : (key -> A -> bool) -> t A -> t A * t A.
+  (** [partition p m] returns a pair of maps [(m1, m2)], where
+  [m1] is the map of all the elements of [m] that satisfy the
+  predicate [p], and [m2] is the map of all the elements of
+  [m] that do not satisfy [p]. *)
 
-    (* TODO: Does not exist in FSet, OCaml has merge. What to do? *)
-    (*
-    Parameter union : t A -> t A -> t A.
-    (** Set union. *)
+  Parameter cardinal : t A -> nat.
+  (** Return the number of elements of a map. *)
 
-    Parameter inter : t -> t -> t.
-    (** Set intersection. *)
+  Parameter elements : t A -> list (key * A).
+  (** Return the list of all keys and values of the given map,
+  in any order. *)
 
-    Parameter diff : t -> t -> t.
-    (** Set difference. *)
-    *)
-
-    Parameter subset : (A -> A -> bool) -> t A -> t A -> bool.
-    (** [subset val_eq m1 m2] tests whether the map [m1] is a subset of
-        the map [m2], where the values [v1] and [v2] for a common key [k]
-        must be equal according to [val_eq]. *)
-
-    Parameter for_all : (key -> A -> bool) -> t A -> bool.
-    (** [for_all p m] checks if all elements of the map [m]
-        satisfy the predicate [p]. *)
-
-    Parameter exists_ : (key -> A -> bool) -> t A -> bool.
-    (** [exists p m] checks if at least one element of
-        the map [m] satisfies the predicate [p]. *)
-
-    Parameter filter : (key -> A -> bool) -> t A -> t A.
-    (** [filter p m] returns the map of all elements in [m]
-        that satisfy predicate [p]. *)
-
-    Parameter partition : (key -> A -> bool) -> t A -> t A * t A.
-    (** [partition p m] returns a pair of maps [(m1, m2)], where
-        [m1] is the map of all the elements of [m] that satisfy the
-        predicate [p], and [m2] is the map of all the elements of
-        [m] that do not satisfy [p]. *)
-
-    Parameter choose : t A -> option (key * A).
-    (** Return one key and value of the given map, or [None] if
-        the map is empty. Which key is chosen is unspecified.
-        Equal maps could return different elements. *)
-  End Types.
+  Parameter choose : t A -> option (key * A).
+  (** Return one key and value of the given map, or [None] if
+  the map is empty. Which key is chosen is unspecified.
+  Equal maps could return different elements. *)
+  End Foo.
 End HasWOps.
 
 
@@ -162,125 +134,101 @@ Module Type WMapsOn (E : DecidableType).
   (** First, we ask for all the functions *)
   Include WOps E.
 
+  Section Foo.
+  Variable A : Type.
+
   (** Logical predicates *)
-  Section LogPred.
-    Variable A : Type.
 
-    Parameter MapsTo : key -> A -> t A -> Prop.
-    Declare Instance MapsTo_compat : Proper (E.eq==>eq==>eq==>iff) MapsTo.
+  Parameter MapsTo : key -> A -> t A -> Prop.
+  Declare Instance MapsTo_compat : Proper (E.eq==>eq==>eq==>iff) MapsTo.
 
-    Definition In (k:key)(m: t A) : Prop := exists e:A, MapsTo k e m.
-    Definition Empty m := forall k a, ~ MapsTo k a m.
+  Definition In (k:key)(m: t A) : Prop := exists e:A, MapsTo k e m.
+  Definition Empty m := forall k a, ~ MapsTo k a m.
 
-    Definition eq_key (p p':key*A) := E.eq (fst p) (fst p').
-    Definition eq_key_elt (p p':key*A) :=
-      E.eq (fst p) (fst p') /\ (snd p) = (snd p').
+  Definition eq_key (p p':key*A) := E.eq (fst p) (fst p').
+  Definition eq_key_elt (p p':key*A) :=
+          E.eq (fst p) (fst p') /\ (snd p) = (snd p').
 
 
-    (** Equality of maps *)
+  (* TODO: Copy explanation from FMap *)
+  Definition Equal m m' := forall k, @find A k m = find k m'.
+  Definition Equiv (eq_elt: A -> A -> Prop) m m' :=
+         (forall k, In k m <-> In k m') /\
+         (forall k e e', MapsTo k e m -> MapsTo k e' m' -> eq_elt e e').
+  Definition Equivb (cmp: A -> A -> bool) := Equiv (Cmp cmp).
 
-    (** Caveat: there are at least three distinct equality predicates on maps.
-      - The simpliest (and maybe most natural) way is to consider keys up to
-        their equivalence [E.eq], but elements up to Leibniz equality, in
-        the spirit of [eq_key_elt] above. This leads to predicate [Equal].
-      - Unfortunately, this [Equal] predicate can't be used to describe
-        the [equal] function, since this function (for compatibility with
-        ocaml) expects a boolean comparison [cmp] that may identify more
-        elements than Leibniz. So logical specification of [equal] is done
-        via another predicate [Equivb]
-      - This predicate [Equivb] is quite ad-hoc with its boolean [cmp],
-        it can be generalized in a [Equiv] expecting a more general
-        (possibly non-decidable) equality predicate on elements *)
+  Definition For_all (P : key -> A -> Prop) m := forall k a, MapsTo k a m -> P k a.
+  Definition Exists (P : key -> A -> Prop) m := exists k a, MapsTo k a m /\ P k a.
 
-    Definition Equal m m' := forall k, @find A k m = find k m'.
-    Definition Equiv (eq_elt: A -> A -> Prop) m m' :=
-      (forall k, In k m <-> In k m') /\
-      (forall k e e', MapsTo k e m -> MapsTo k e' m' -> eq_elt e e').
-    Definition Equivb (cmp: A -> A -> bool) := Equiv (Cmp cmp).
+  Definition eq : t A -> t A -> Prop := Equal.
+ 
+  (*
+  Include IsEq. (** [eq] is obviously an equivalence, for subtyping only *)
+  Include HasEqDec.
+  *)
 
-    Definition For_all (P : key -> A -> Prop) m := forall k a, MapsTo k a m -> P k a.
-    Definition Exists (P : key -> A -> Prop) m := exists k a, MapsTo k a m /\ P k a.
+  (** Specifications of map operators *)
 
-    Definition eq : t A -> t A -> Prop := Equal.
+  Section Spec.
 
-    (** Including IsEq and HasEqDec more hassle than it's worth:
-        can't instantiate these higher-order module types w/ "yourself",
-        since [t] has wrong type ([Type -> Type] instead of [Type]), and
-        creating a new module type parametrized by A -- how exactly
-        would we make that work, even? -- is just not worth the work.
+  Variable m m': t A.
+  Variable k k' : key.
+  Variable v v' : A.
+  Variable f : key -> A -> bool.
+  Notation compatb := (Proper (E.eq==>Logic.eq==>Logic.eq)) (only parsing).
 
-        Contents copied outright instead *)
-    Global Declare Instance eq_equiv : Equivalence eq.
-    Parameter eq_dec : forall x y : t A, { eq x y } + { ~ eq x y }.
+  Parameter MapsTo_spec : E.eq k k' -> MapsTo k v m -> MapsTo k' v m.
 
-    (** Specifications of map operators *)
+  Parameter unique: MapsTo k v m -> MapsTo k v' m -> v = v'.
 
-    Section Spec.
+  Parameter find_spec : find k m = Some v <-> MapsTo k v m.
+  Parameter mem_spec : mem k m = true <-> In k m.
+  Section EqSpec.
+     Variable cmp : A -> A -> bool.
+     Parameter equal_1 : Equivb cmp m m' -> equal cmp m m' = true.
+     Parameter equal_2 : equal cmp m m' = true -> Equivb cmp m m'.
+  End EqSpec.
 
-      Variable m m' m'': t A.
-      Variable k k' k'': key.
-      Variable v v' v'': A.
-      Variable f : key -> A -> bool.
-      Notation compatb := (Proper (E.eq==>Logic.eq==>Logic.eq)) (only parsing).
+  Parameter empty_spec : Empty (empty A).
+  Parameter is_empty_spec : is_empty m = true <-> Empty m.
+  (* Parameter add_spec : In k1 (add k2 v m) <-> E.eq y x \/ In y m. *)
+  Parameter add_spec1: E.eq k k' -> MapsTo k v (add k' v m).
+  Parameter add_spec2: ~ E.eq k k' -> (MapsTo k v (add k' v' m) <-> MapsTo k v m).
 
-      (* Keys in the map are unique *)
-      (* TODO: is this not elements_spec2w? *)
-      Parameter unique: MapsTo k v m -> MapsTo k v' m -> v = v'.
+  Parameter remove_spec1: E.eq k k' -> ~ In k (remove k' m).
+  Parameter remove_spec2: ~ E.eq k k' -> MapsTo k' v (remove k m) <-> MapsTo k' v m.
 
-      Parameter MapsTo_spec : E.eq k k' -> MapsTo k v m -> MapsTo k' v m.
+  Parameter singleton_spec: E.eq k k' <-> MapsTo k v (singleton k' v).
 
-      Parameter find_spec : find k m = Some v <-> MapsTo k v m.
-      Parameter mem_spec : mem k m = true <-> In k m.
-      Section EqSpec.
-        Variable cmp : A -> A -> bool.
-        Parameter equal_spec1 : Equivb cmp m m' -> equal cmp m m' = true.
-        Parameter equal_spec2 : equal cmp m m' = true -> Equivb cmp m m'.
-      End EqSpec.
+  (*
+  Parameter union_spec : In x (union m m') <-> In x m \/ In x m'.
+  Parameter inter_spec : In x (inter m m') <-> In x m /\ In x m'.
+  Parameter diff_spec : In x (diff m m') <-> In x m /\ ~In x m'.
+  *)
 
-      Parameter empty_spec : Empty (empty A).
-      Parameter is_empty_spec : is_empty m = true <-> Empty m.
+  Parameter fold_spec : forall (X : Type) (i : X) (f : key -> A -> X -> X),
+    fold f m i = fold_left (fun a p => f (fst p) (snd p) a ) (elements m) i.
+  Parameter cardinal_spec : cardinal m = length (elements m).
+  Parameter filter_spec : compatb f ->
+    (MapsTo k v (filter f m) <-> MapsTo k v m /\ f k v = true).
+  Parameter for_all_spec : compatb f ->
+    (for_all f m = true <-> For_all (fun k v => f k v = true) m).
+  Parameter exists_spec : compatb f ->
+    (exists_ f m = true <-> Exists (fun k v => f k v = true) m).
+  Parameter partition_spec1 : compatb f ->
+    Equal (fst (partition f m)) (filter f m).
+  Parameter partition_spec2 : compatb f ->
+    Equal (snd (partition f m)) (filter (fun k x => negb (f k x)) m).
+  
+  Parameter elements_spec1 : InA eq_key_elt (k, v) (elements m) <-> MapsTo k v m.
+  (** When compared with ordered maps, here comes the only
+      property that is really weaker: *)
+  Parameter elements_spec2w : NoDupA eq_key (elements m).
+  Parameter choose_spec1 : choose m = Some (k,v) -> MapsTo k v m.
+  Parameter choose_spec2 : choose m = None -> Empty m.
 
-      Parameter add_spec1: E.eq k k' -> MapsTo k v (add k' v m).
-      Parameter add_spec2: ~ E.eq k k' -> (MapsTo k v (add k' v' m) <-> MapsTo k v m).
-
-      Parameter remove_spec1: E.eq k k' -> ~ In k (remove k' m).
-      Parameter remove_spec2: ~ E.eq k k' -> (MapsTo k' v (remove k m) <-> MapsTo k' v m).
-
-
-      Parameter fold_spec : forall (X : Type) (i : X) (f : key -> A -> X -> X),
-                              fold f m i = fold_left (fun a p => f (fst p) (snd p) a ) (elements m) i.
-      Parameter cardinal_spec : cardinal m = length (elements m).
-
-      Parameter elements_spec1 : InA eq_key_elt (k, v) (elements m) <-> MapsTo k v m. 
-      (** When compared with ordered maps, here comes the only
-          property that is really weaker: *)
-      Parameter elements_spec2w : NoDupA eq_key (elements m).
-
-      (* TODO: all of these are new when comparing to FMap *)
-      Parameter singleton_spec: E.eq k k' <-> MapsTo k v (singleton k' v).
-
-      (*
-      Parameter union_spec : In x (union m m') <-> In x m \/ In x m'.
-      Parameter inter_spec : In x (inter m m') <-> In x m /\ In x m'.
-      Parameter diff_spec : In x (diff m m') <-> In x m /\ ~In x m'.
-      *)
-      (* TODO: Isn't subset_spec missing? *)
-      Parameter filter_spec : compatb f ->
-                              (MapsTo k v (filter f m) <-> MapsTo k v m /\ f k v = true).
-      Parameter for_all_spec : compatb f ->
-                               (for_all f m = true <-> For_all (fun k v => f k v = true) m).
-      Parameter exists_spec : compatb f ->
-                              (exists_ f m = true <-> Exists (fun k v => f k v = true) m).
-      Parameter partition_spec1 : compatb f ->
-                                  Equal (fst (partition f m)) (filter f m).
-      Parameter partition_spec2 : compatb f ->
-                                  Equal (snd (partition f m)) (filter (fun k x => negb (f k x)) m).
-      
-      Parameter choose_spec1 : choose m = Some (k,v) -> MapsTo k v m.
-      Parameter choose_spec2 : choose m = None -> Empty m.
-
-    End Spec.
-  End LogPred.
+  End Spec.
+  End Foo.
 
 End WMapsOn.
 
@@ -300,22 +248,24 @@ End WMaps.
     and some stronger specifications for other functions. *)
 
 Module Type HasOrdOps (Import T:TypElt).
-  Section LogPred.
-    Variable A : Type.
+  Section Foo.
+  Variable A : Type.
 
-    Parameter compare : t A -> t A -> comparison.
-    (** Total ordering between maps. Can be used as the ordering function
-        for doing maps of maps. *)
+  (* TODO: Does this make sense? We'd have to compare values
+  Parameter compare : t A -> t A -> comparison.
+  *)
+  (** Total ordering between maps. Can be used as the ordering function
+  for doing maps of maps. *)
 
-    Parameter min_elt : t A -> option (key * A).
-    (** Return the smallest key and the associated value of the given map
-        (with respect to the [E.compare] ordering),
-        or [None] if the map is empty. *)
+  Parameter min_elt : t A -> option (key * A).
+  (** Return the smallest key and the associated value of the given map
+  (with respect to the [E.compare] ordering),
+  or [None] if the map is empty. *)
 
-    Parameter max_elt : t A -> option (key * A).
-    (** Same as [min_elt], but returns the largest key and the associated
-        value of the given map. *)
-  End LogPred.
+  Parameter max_elt : t A -> option (key * A).
+  (** Same as [min_elt], but returns the largest key and the associated
+  value of the given map. *)
+  End Foo.
 End HasOrdOps.
 
 Module Type Ops (E : OrderedType) := WOps E <+ HasOrdOps.
@@ -324,37 +274,39 @@ Module Type Ops (E : OrderedType) := WOps E <+ HasOrdOps.
 Module Type MapsOn (E : OrderedType).
 
   Include WMapsOn E <+ HasOrdOps.
+  (* TODO: type of HasLt not matched (like Eq above)
+  Include WMapsOn E <+ HasOrdOps <+ HasLt <+ IsStrOrder.
+  *)
 
   Section Spec.
-    Variable A : Type.
-    Variable m m': t A.
-    Variable k k' : key.
-    Variable v v' : A.
+  Variable A : Type.
+  Variable m m': t A.
+  Variable k k' : key.
+  Variable v v' : A.
 
-    Parameter lt: t A -> t A -> Prop.
-    Global Declare Instance lt_strorder : StrictOrder lt.
-    Global Declare Instance lt_compat : Proper (Logic.eq==>Logic.eq==>iff) lt.
+  (* TODO: Requires HasLt or IsStrOrder
+  Parameter compare_spec : CompSpec eq lt m m' (compare m m').
+  *)
 
-    Parameter compare_spec : CompSpec Logic.eq lt m m' (compare m m').
+  (** Additional specification of [elements] *)
+  Parameter elements_spec2 : sort (fun p1 p2 => E.lt (fst p1) (fst p2)) (elements m).
 
-    (** Additional specification of [elements] *)
-    Parameter elements_spec2 : sort (fun p1 p2 => E.lt (fst p1) (fst p2)) (elements m).
+  (** Remark: since [fold] is specified via [elements], this stronger
+   specification of [elements] has an indirect impact on [fold],
+   which can now be proved to receive elements in increasing order.
+  *)
 
-    (** Remark: since [fold] is specified via [elements], this stronger
-        specification of [elements] has an indirect impact on [fold],
-        which can now be proved to receive elements in increasing order.*)
+  Parameter min_elt_spec1 : min_elt m = Some (k,v) -> MapsTo k v m.
+  Parameter min_elt_spec2 : min_elt m = Some (k,v) -> MapsTo k' v' m -> ~ E.lt k' k.
+  Parameter min_elt_spec3 : min_elt m = None -> Empty m.
 
-    Parameter min_elt_spec1 : min_elt m = Some (k,v) -> MapsTo k v m.
-    Parameter min_elt_spec2 : min_elt m = Some (k,v) -> MapsTo k' v' m -> ~ E.lt k' k.
-    Parameter min_elt_spec3 : min_elt m = None -> Empty m.
+  Parameter max_elt_spec1 : max_elt m = Some (k,v) -> MapsTo k v m.
+  Parameter max_elt_spec2 : max_elt m = Some (k,v) -> MapsTo k' v' m -> ~ E.lt k k'.
+  Parameter max_elt_spec3 : max_elt m = None -> Empty m.
 
-    Parameter max_elt_spec1 : max_elt m = Some (k,v) -> MapsTo k v m.
-    Parameter max_elt_spec2 : max_elt m = Some (k,v) -> MapsTo k' v' m -> ~ E.lt k k'.
-    Parameter max_elt_spec3 : max_elt m = None -> Empty m.
-
-    (** Additional specification of [choose] *)
-    Parameter choose_spec3 : choose m = Some (k, v) -> choose m' = Some (k', v') ->
-                             Equal m m' -> E.eq k k'.
+  (** Additional specification of [choose] *)
+  Parameter choose_spec3 : choose m = Some (k, v) -> choose m' = Some (k', v') ->
+    Equal m m' -> E.eq k k'.
 
   End Spec.
 
@@ -449,119 +401,97 @@ Module Type WRawMaps (E : DecidableType).
   Parameter isok : forall A, t A -> bool.
   Declare Instance isok_Ok {A : Type} (s : t A) `(isok s = true) : Ok s | 10.
 
+  Section Foo.
+  Variable A : Type.
+
   (** Logical predicates *)
-  Section LogPred.
-    Variable A : Type.
 
-    Parameter MapsTo : key -> A -> t A -> Prop.
-    Declare Instance MapsTo_compat : Proper (E.eq==>eq==>eq==>iff) MapsTo.
+  Parameter MapsTo : key -> A -> t A -> Prop.
+  Declare Instance MapsTo_compat : Proper (E.eq==>eq==>eq==>iff) MapsTo.
 
-    Definition In (k:key)(m: t A) : Prop := exists e:A, MapsTo k e m.
-    Definition Empty m := forall k a, ~ MapsTo k a m.
+  Definition In (k:key)(m: t A) : Prop := exists e:A, MapsTo k e m.
+  Definition Empty m := forall k a, ~ MapsTo k a m.
 
-    Definition eq_key (p p':key*A) := E.eq (fst p) (fst p').
-    Definition eq_key_elt (p p':key*A) :=
-      E.eq (fst p) (fst p') /\ (snd p) = (snd p').
+  Definition eq_key (p p':key*A) := E.eq (fst p) (fst p').
+  Definition eq_key_elt (p p':key*A) :=
+          E.eq (fst p) (fst p') /\ (snd p) = (snd p').
 
 
-    Definition Equal m m' := forall k, @find A k m = find k m'.
-    Definition Equiv (eq_elt: A -> A -> Prop) m m' :=
-      (forall k, In k m <-> In k m') /\
-      (forall k e e', MapsTo k e m -> MapsTo k e' m' -> eq_elt e e').
-    Definition Equivb (cmp: A -> A -> bool) := Equiv (Cmp cmp).
+  Definition Equal m m' := forall k, @find A k m = find k m'.
+  Definition Equiv (eq_elt: A -> A -> Prop) m m' :=
+         (forall k, In k m <-> In k m') /\
+         (forall k e e', MapsTo k e m -> MapsTo k e' m' -> eq_elt e e').
+  Definition Equivb (cmp: A -> A -> bool) := Equiv (Cmp cmp).
 
-    Definition For_all (P : key -> A -> Prop) m := forall k a, MapsTo k a m -> P k a.
-    Definition Exists (P : key -> A -> Prop) m := exists k a, MapsTo k a m /\ P k a.
+  Definition For_all (P : key -> A -> Prop) m := forall k a, MapsTo k a m -> P k a.
+  Definition Exists (P : key -> A -> Prop) m := exists k a, MapsTo k a m /\ P k a.
 
-    Definition eq : t A -> t A -> Prop := Equal.
-    
-    Declare Instance eq_equiv : Equivalence eq.
+  Definition eq : t A -> t A -> Prop := Equal.
+ 
+  Declare Instance eq_equiv : Equivalence eq.
 
-    (** Now, the specifications, with constraints on the input sets. *)
-    Section Spec.
-      Variable s s': t A.
-      Variable k k' : key.
-      Variable v v' : A.
-      Variable f : key -> A -> bool.
-      Notation compatb := (Proper (E.eq==>Logic.eq==>Logic.eq)) (only parsing).
+  (** Now, the specifications, with constraints on the input sets. *)
+  Section Spec.
+  Variable s s': t A.
+  Variable k k' : key.
+  Variable v v' : A.
+  Variable f : key -> A -> bool.
+  Notation compatb := (Proper (E.eq==>Logic.eq==>Logic.eq)) (only parsing).
 
-      Parameter mem_spec : forall `{Ok A s}, mem k s = true <-> In k s.
+  Parameter mem_spec : forall `{Ok A s}, mem k s = true <-> In k s.
 
-      Section EqSpec.
-        Variable cmp : A -> A -> bool.
-        Parameter equal_1 : 
-          forall `{Ok A s, Ok A s'},
-            Equivb cmp s s' -> equal cmp s s' = true.
-        Parameter equal_2 :
-          forall `{Ok A s, Ok A s'},
-            equal cmp s s' = true -> Equivb cmp s s'.
-      End EqSpec.
+ Section EqSpec.
+     Variable cmp : A -> A -> bool.
+     Parameter equal_1 : 
+       forall `{Ok A s, Ok A s'},
+       Equivb cmp s s' -> equal cmp s s' = true.
+     Parameter equal_2 :
+       forall `{Ok A s, Ok A s'},
+       equal cmp s s' = true -> Equivb cmp s s'.
+  End EqSpec.
 
-      Parameter empty_spec : Empty (empty A).
-      Parameter is_empty_spec : is_empty s = true <-> Empty s.
-      Parameter add_spec1: forall `{Ok A s},
-                             E.eq k k' -> MapsTo k v (add k' v s).
-      Parameter add_spec2: forall `{Ok A s},
-                             ~ E.eq k k' -> (MapsTo k v (add k' v' s) <-> MapsTo k v s).
-      Parameter remove_spec1: forall `{Ok A s},
-                                E.eq k k' -> ~ In k (remove k' s).
-      Parameter remove_spec2: forall `{Ok A s},
-                                ~ E.eq k k' -> (MapsTo k' v (remove k s) <-> MapsTo k' v s).
-      Parameter singleton_spec :  E.eq k k' <-> MapsTo k v (singleton k' v).
-      (* TODO set operations nor usefull for maps 
-      Parameter union_spec : forall `{Ok s, Ok s'},
-        In x (union s s') <-> In x s \/ In x s'.
-      Parameter inter_spec : forall `{Ok s, Ok s'},
-        In x (inter s s') <-> In x s /\ In x s'.
-      Parameter diff_spec : forall `{Ok s, Ok s'},
-        In x (diff s s') <-> In x s /\ ~In x s'.
-       *)
-      Parameter fold_spec : forall (X : Type) (i : X) (f : key -> A -> X -> X),
-                              fold f s i = fold_left (fun (x:X) (p:key*A) => f (fst p) (snd p) x ) (elements s) i.
-      Parameter cardinal_spec : forall `{Ok A s},
-                                  cardinal s = length (elements s).
-      Parameter filter_spec : compatb f ->
-                              (MapsTo k v (filter f s) <-> MapsTo k v s /\ f k v = true).
-      Parameter for_all_spec : compatb f ->
-                               (for_all f s = true <-> For_all (fun x a => f x a = true) s).
-      Parameter exists_spec : compatb f ->
-                              (exists_ f s = true <-> Exists (fun x a => f x a = true) s).
-      Parameter partition_spec1 : compatb f ->
-                                  Equal (fst (partition f s)) (filter f s).
-      Parameter partition_spec2 : compatb f ->
-                                  Equal (snd (partition f s)) (filter (fun x a => negb (f x a)) s).
-      Parameter elements_spec1 : InA eq_key_elt (k, v) (elements s) <-> MapsTo k v s.
-      (** When compared with ordered sets, here comes the only
+  Parameter empty_spec : Empty (empty A).
+  Parameter is_empty_spec : is_empty s = true <-> Empty s.
+  Parameter add_spec1: forall `{Ok A s},
+     E.eq k k' -> MapsTo k v (add k' v s).
+  Parameter add_spec2: forall `{Ok A s},
+     ~ E.eq k k' -> (MapsTo k v (add k' v' s) <-> MapsTo k v s).
+  Parameter remove_spec1: forall `{Ok A s},
+    E.eq k k' -> ~ In k (remove k' s).
+  Parameter remove_spec2: forall `{Ok A s},
+    ~ E.eq k k' -> MapsTo k' v (remove k s) <-> MapsTo k' v s.
+  Parameter singleton_spec :  E.eq k k' <-> MapsTo k v (singleton k' v).
+  (* TODO set operations nor usefull for maps 
+  Parameter union_spec : forall `{Ok s, Ok s'},
+    In x (union s s') <-> In x s \/ In x s'.
+  Parameter inter_spec : forall `{Ok s, Ok s'},
+    In x (inter s s') <-> In x s /\ In x s'.
+  Parameter diff_spec : forall `{Ok s, Ok s'},
+    In x (diff s s') <-> In x s /\ ~In x s'.
+  *)
+  Parameter fold_spec : forall (X : Type) (i : X) (f : key -> A -> X -> X),
+    fold f s i = fold_left (fun (x:X) (p:key*A) => f (fst p) (snd p) x ) (elements s) i.
+  Parameter cardinal_spec : forall `{Ok A s},
+    cardinal s = length (elements s).
+  Parameter filter_spec : compatb f ->
+    (MapsTo k v (filter f s) <-> MapsTo k v s /\ f k v = true).
+  Parameter for_all_spec : compatb f ->
+    (for_all f s = true <-> For_all (fun x a => f x a = true) s).
+  Parameter exists_spec : compatb f ->
+    (exists_ f s = true <-> Exists (fun x a => f x a = true) s).
+  Parameter partition_spec1 : compatb f ->
+    Equal (fst (partition f s)) (filter f s).
+  Parameter partition_spec2 : compatb f ->
+    Equal (snd (partition f s)) (filter (fun x a => negb (f x a)) s).
+  Parameter elements_spec1 : InA eq_key_elt (k, v) (elements s) <-> MapsTo k v s.
+  (** When compared with ordered sets, here comes the only
       property that is really weaker: *)
-      Parameter elements_spec2w : forall `{Ok A s}, NoDupA eq_key (elements s).
-      Parameter choose_spec1 : choose s = Some (k,v) -> MapsTo k v s.
-      Parameter choose_spec2 : choose s = None -> Empty s.
-    End Spec.
-  End LogPred.
+  Parameter elements_spec2w : NoDupA eq_key (elements s).
+  Parameter choose_spec1 : choose s = Some (k,v) -> MapsTo k v s.
+  Parameter choose_spec2 : choose s = None -> Empty s.
 
-  (* TODO: Should this be in the section? *)
-  (** Specification of [map] *)
-  Parameter map_spec1 : forall (A A':Type)(s: t A)(k:key)(e:A)(f:A->A'),
-                      MapsTo k e s -> MapsTo k (f e) (map f s).
-  Parameter map_spec2 : forall (A A':Type)(s: t A)(k:key)(f:A->A'),
-                      In k (map f s) -> In k s.
-
-  (** Specification of [mapi] *)
-  Parameter mapi_spec1 : forall (A A':Type)(m: t A)(x:key)(e:A)(f:key->A->A'), 
-                       MapsTo x e m -> exists y, E.eq y x /\ MapsTo x (f y e) (mapi f m).
-  Parameter mapi_spec2 : forall (A A':Type)(m: t A)(x:key)
-                            (f:key->A->A'), In x (mapi f m) -> In x m.
-
-  (** Specification of [map2] *)
-  Parameter map2_spec1 : forall (A A' A'':Type)(m: t A)(m': t A')
-	                        (x:key)(f:option A->option A'->option A''),
-	                   In x m \/ In x m' ->
-                       find x (map2 f m m') = f (find x m) (find x m').
-
-  Parameter map2_spec2 : forall (A A' A'':Type)(m: t A)(m': t A')
-	                        (x:key)(f:option A->option A'->option A''),
-                       In x (map2 f m m') -> In x m \/ In x m'.
-
+  End Spec.
+  End Foo.
 
   (** All operations are compatible with the well-formed predicate. *)
   (* This needs to live outside of the Section with Variable A *)
@@ -569,7 +499,7 @@ Module Type WRawMaps (E : DecidableType).
   Declare Instance add_ok A s x a `(Ok A s) : Ok (add x a s).
   Declare Instance remove_ok A s x `(Ok A s) : Ok (remove x s).
   Declare Instance singleton_ok A x (a : A) : Ok (singleton x a).
-  (* Set functionality not usefull in map
+  (* Set functionality not usefull in MAP
   Declare Instance union_ok s s' `(Ok s, Ok s') : Ok (union s s').
   Declare Instance inter_ok s s' `(Ok s, Ok s') : Ok (inter s s').
   Declare Instance diff_ok s s' `(Ok s, Ok s') : Ok (diff s s').
@@ -578,10 +508,6 @@ Module Type WRawMaps (E : DecidableType).
   Declare Instance partition_ok1 A s f `(Ok A s) : Ok (fst (partition f s)).
   Declare Instance partition_ok2 A s f `(Ok A s) : Ok (snd (partition f s)).
 
-  Declare Instance map_ok A A' s (g: A -> A') `(Ok A s): Ok (map g s).
-  Declare Instance mapi_ok A A' s (g: key -> A -> A') `(Ok A s): Ok (mapi g s).
-  Declare Instance map2_ok A A' A'' s s' 
-          (g: option A -> option A' -> option A'') `(Ok A s): Ok (map2 g s s').
 
 End WRawMaps.
 
@@ -599,183 +525,157 @@ Module WRaw2MapsOn (E:DecidableType)(M:WRawMaps E) <: WMapsOn E.
  Arguments Mkt {A} this {is_ok}.
  Hint Resolve is_ok : typeclass_instances.
 
- Section Defs.
-   Variables A A' A'': Type.
+ Section Foo.
+ Variable A : Type.
 
-   Definition mem (x : key)(s : t A) := M.mem x s.
-   Definition find (x : key)(s : t A) := M.find x s.
-   Definition add (x : key) v (s : t A) : t A := Mkt (M.add x v s).
-   Definition singleton (x : key) v : t A := Mkt (M.singleton x v).
-   Definition remove (x : key)(s : t A) : t A := Mkt (M.remove x s).
-   (*
-   Definition union (s s' : t) : t := Mkt (M.union s s').
-   Definition inter (s s' : t) : t := Mkt (M.inter s s').
-   Definition diff (s s' : t) : t := Mkt (M.diff s s').
-    *)
-   Definition equal (f : A -> A -> bool) (s s' : t A) := M.equal f s s'.
-   Definition subset (f : A -> A -> bool) (s s' : t A) := M.subset f s s'.
-   Definition empty : t A := Mkt (M.empty A).
-   Definition is_empty (s : t A) := M.is_empty s.
-   Definition elements (s : t A) : list (key * A) := M.elements s.
-   Definition choose (s : t A) : option (key * A) := M.choose s.
-   Definition fold (X : Type)(f : key -> A -> X -> X)(s : t A) : X -> X := M.fold f s.
-   Definition cardinal (s : t A) := M.cardinal s.
-   Definition filter (f : key -> A -> bool)(s : t A) : t A := Mkt (M.filter f s).
-   Definition for_all (f : key -> A -> bool)(s : t A) := M.for_all f s.
-   Definition exists_ (f : key -> A -> bool)(s : t A) := M.exists_ f s.
-   Definition partition (f : key -> A -> bool)(s : t A) : t A * t A :=
-     let p := M.partition f s in (Mkt (fst p), Mkt (snd p)).
-   Definition map (f: A -> A')(l: t A) : t A' := Mkt (M.map f l).
-   Definition mapi (f: key -> A -> A')(l: t A) : t A' := Mkt (M.mapi f l).
-   Definition map2 (f: option A -> option A' -> option A'')(l0: t A) (l1: t A') : t A'':= 
-     Mkt (M.map2 f l0 l1).
+ Definition mem (x : key)(s : t A) := M.mem x s.
+ Definition find (x : key)(s : t A) := M.find x s.
+ Definition add (x : key) v (s : t A) : t A := Mkt (M.add x v s).
+ Definition singleton (x : key) v : t A := Mkt (M.singleton x v).
+ Definition remove (x : key)(s : t A) : t A := Mkt (M.remove x s).
+ (*
+ Definition union (s s' : t) : t := Mkt (M.union s s').
+ Definition inter (s s' : t) : t := Mkt (M.inter s s').
+ Definition diff (s s' : t) : t := Mkt (M.diff s s').
+ *)
+ Definition equal (f : A -> A -> bool) (s s' : t A) := M.equal f s s'.
+ Definition subset (f : A -> A -> bool) (s s' : t A) := M.subset f s s'.
+ Definition empty : t A := Mkt (M.empty A).
+ Definition is_empty (s : t A) := M.is_empty s.
+ Definition elements (s : t A) : list (key * A) := M.elements s.
+ Definition choose (s : t A) : option (key * A) := M.choose s.
+ Definition fold (X : Type)(f : key -> A -> X -> X)(s : t A) : X -> X := M.fold f s.
+ Definition cardinal (s : t A) := M.cardinal s.
+ Definition filter (f : key -> A -> bool)(s : t A) : t A := Mkt (M.filter f s).
+ Definition for_all (f : key -> A -> bool)(s : t A) := M.for_all f s.
+ Definition exists_ (f : key -> A -> bool)(s : t A) := M.exists_ f s.
+ Definition partition (f : key -> A -> bool)(s : t A) : t A * t A :=
+   let p := M.partition f s in (Mkt (fst p), Mkt (snd p)).
 
-   Definition MapsTo (x : key) (v : A) (s : t A) := M.MapsTo x v s.(this).
-   Definition In (k:key)(m: t A) : Prop := exists e:A, MapsTo k e m.
-   Definition Empty m := forall k a, ~ MapsTo k a m.
 
-   Definition Equal m m' := forall k, find k m = find k m'.
-   Definition Equiv (eq_elt: A -> A -> Prop) m m' :=
-     (forall k, In k m <-> In k m') /\
-     (forall k e e', MapsTo k e m -> MapsTo k e' m' -> eq_elt e e').
-   Definition Equivb (cmp: A -> A -> bool) := Equiv (Cmp cmp).
+ Definition MapsTo (x : key) (v : A) (s : t A) := M.MapsTo x v s.(this).
+ Definition In (k:key)(m: t A) : Prop := exists e:A, MapsTo k e m.
+ Definition Empty m := forall k a, ~ MapsTo k a m.
 
-   Definition For_all (P : key -> A -> Prop) m := forall k a, MapsTo k a m -> P k a.
-   Definition Exists (P : key -> A -> Prop) m := exists k a, MapsTo k a m /\ P k a.
+ Definition Equal m m' := forall k, find k m = find k m'.
+ Definition Equiv (eq_elt: A -> A -> Prop) m m' :=
+         (forall k, In k m <-> In k m') /\
+         (forall k e e', MapsTo k e m -> MapsTo k e' m' -> eq_elt e e').
+ Definition Equivb (cmp: A -> A -> bool) := Equiv (Cmp cmp).
 
-   Definition eq_key (p p':key*A) := E.eq (fst p) (fst p').
-   Definition eq_key_elt (p p':key*A) :=
-     E.eq (fst p) (fst p') /\ (snd p) = (snd p').
+ Definition For_all (P : key -> A -> Prop) m := forall k a, MapsTo k a m -> P k a.
+ Definition Exists (P : key -> A -> Prop) m := exists k a, MapsTo k a m /\ P k a.
 
-   Instance MapsTo_compat : Proper (E.eq==>eq==>eq==>iff) MapsTo.
-   Proof. repeat red. intros; apply M.MapsTo_compat; congruence. Qed.
 
-   Definition eq : t A -> t A -> Prop := Equal.
+ Definition eq_key (p p':key*A) := E.eq (fst p) (fst p').
+ Definition eq_key_elt (p p':key*A) :=
+          E.eq (fst p) (fst p') /\ (snd p) = (snd p').
 
-   Instance eq_equiv : Equivalence eq.
-   split; try firstorder. unfold Transitive; unfold eq; unfold Equal.
-   firstorder; rewrite H; auto.
-   Qed.
 
-   (* TODO: doesn't this proof requre comparison for equal? *)
-   Definition eq_dec : forall (s s':t A), { eq s s' }+{ ~eq s s' }.
-   Admitted.
-   (*
-   Proof.
-    intros (s,Hs) (s',Hs').
-    change ({M.Equal s s'}+{~M.Equal s s'}).
-    destruct (M.equal s s') eqn:H; [left|right];
-     rewrite <- M.equal_spec; congruence.
-   Defined.
-   *)
 
-   Section Spec.
-     Variable s s' : t A.
-     Variable k k' : key.
-     Variable v v' : A.
-     Variable f : key -> A -> bool. 
-     Variable g: A -> A'.
-     Variable gi : key -> A -> A'.
-     Variable g2 : option A -> option A' -> option A''.
-     Variable cmp : A -> A -> bool.
-     Notation compatb := (Proper (E.eq==>Logic.eq==>Logic.eq)) (only parsing).
+ Instance MapsTo_compat : Proper (E.eq==>eq==>eq==>iff) MapsTo.
+ Proof. repeat red. intros; apply M.MapsTo_compat; congruence. Qed.
 
-     Lemma MapsTo_spec : E.eq k k' -> MapsTo k v s -> MapsTo k' v s.
-     Admitted.
+ Definition eq : t A -> t A -> Prop := Equal.
 
-     Lemma unique: MapsTo k v s -> MapsTo k v' s -> v = v'.
-     Admitted.
+ Instance eq_equiv : Equivalence eq.
+ (* Proof. firstorder. Qed.*)
+ Admitted.
 
-     Lemma find_spec : find k s = Some v <-> MapsTo k v s.
-     Admitted.
+ Definition eq_dec : forall (s s':t A), { eq s s' }+{ ~eq s s' }.
+ Admitted.
+ (*
+ Proof.
+  intros (s,Hs) (s',Hs').
+  change ({M.Equal s s'}+{~M.Equal s s'}).
+  destruct (M.equal s s') eqn:H; [left|right];
+   rewrite <- M.equal_spec; congruence.
+ Defined.
+ *)
 
-     Lemma mem_spec : mem k s = true <-> In k s.
-     Proof. exact (@M.mem_spec _ _ _ _). Qed.
-     Lemma equal_spec1 : Equivb cmp s s' -> equal cmp s s' = true.
-     Proof. exact (@M.equal_1 _ _ _ _ _ _). Qed.
-     Lemma equal_spec2 : equal cmp s s' = true -> Equivb cmp s s'.
-     Proof. exact (@M.equal_2 _ _ _ _ _ _). Qed.
-     (*
-     Lemma subset_spec : subset s s' = true <-> Subset s s'.
-     Proof. exact (@M.subset_spec _ _ _ _). Qed.
-     *)
-     Lemma empty_spec : Empty empty.
-     Proof. exact (@M.empty_spec _). Qed.
-     Lemma is_empty_spec : is_empty s = true <-> Empty s.
-     Proof. exact (@M.is_empty_spec _ _). Qed.
-     Lemma add_spec1 : E.eq k k' -> MapsTo k v (add k' v s).
-     Proof. exact (@M.add_spec1 _ _ _ _ _ _). Qed.
-     Lemma add_spec2 : ~ E.eq k k' -> (MapsTo k v (add k' v' s) <-> MapsTo k v s).
-     Proof. exact (@M.add_spec2 _ _ _ _ _ _ _). Qed.
+ Section Spec.
+  Variable s s' : t A.
+  Variable k k' : key.
+  Variable v v' : A.
+  Variable f : key -> A -> bool. 
+  Variable cmp : A -> A -> bool.
+  Notation compatb := (Proper (E.eq==>Logic.eq==>Logic.eq)) (only parsing).
 
-     Lemma remove_spec1:  E.eq k k' -> ~ In k (remove k' s).
-     Proof. exact (@M.remove_spec1 _ _ _ _ _). Qed.
-     Lemma remove_spec2: ~ E.eq k k' -> (MapsTo k' v (remove k s) <-> MapsTo k' v s).
-     Proof. exact (@M.remove_spec2 _ _ _ _ _ _). Qed.
-     Lemma singleton_spec : E.eq k k' <-> MapsTo k v (singleton k' v).
-     Proof. exact (@M.singleton_spec _ _ _ _). Qed.
-     (*
-     Lemma union_spec : In x (union s s') <-> In x s \/ In x s'.
-     Proof. exact (@M.union_spec _ _ _ _ _). Qed.
-     Lemma inter_spec : In x (inter s s') <-> In x s /\ In x s'.
-     Proof. exact (@M.inter_spec _ _ _ _ _). Qed.
-     Lemma diff_spec : In x (diff s s') <-> In x s /\ ~In x s'.
-     Proof. exact (@M.diff_spec _ _ _ _ _). Qed.
-     *)
-     Lemma fold_spec : forall (X : Type) (i : X) (f : key -> A -> X -> X),
-                         fold f s i =
-                         fold_left (fun (x : X) (p : key * A) => f (fst p) (snd p) x) (elements s) i.
-     Proof. exact (@M.fold_spec _ _). Qed.
-     Lemma cardinal_spec : cardinal s = length (elements s).
-     Proof. exact (@M.cardinal_spec _ s _). Qed.
-     Lemma filter_spec : compatb f ->
-                         (MapsTo k v (filter f s) <-> MapsTo k v s /\ f k v = true).
-     Proof. exact (@M.filter_spec _ _ _ _  _). Qed.
-     Lemma for_all_spec : compatb f ->
-                          (for_all f s = true <-> For_all (fun (x : key) (a : A) => f x a = true) s).
-     Proof. exact (@M.for_all_spec _ _ _). Qed.
-     Lemma exists_spec : compatb f ->
-                         (exists_ f s = true <-> Exists (fun x a => f x a = true) s).
-     Proof. exact (@M.exists_spec _ _ _). Qed.
-     Lemma partition_spec1 : compatb f -> Equal (fst (partition f s)) (filter f s).
-     Proof. exact (@M.partition_spec1 _ _ _). Qed.
-     Lemma partition_spec2 : compatb f ->
-                             Equal (snd (partition f s)) (filter (fun x a => negb (f x a)) s).
-     Proof. exact (@M.partition_spec2 _ _ _). Qed.
-     Lemma elements_spec1 :
-       InA eq_key_elt (k, v) (elements s) <-> MapsTo k v s.
-     Proof. exact (@M.elements_spec1 _ _ _ _). Qed.
-     Lemma elements_spec2w : NoDupA eq_key (elements s).
-     Proof. exact (@M.elements_spec2w _ _ _). Qed.
-     Lemma choose_spec1 : choose s = Some (k,v) -> MapsTo k v s.
-     Proof. exact (@M.choose_spec1 _ _ _ _). Qed.
-     Lemma choose_spec2 : choose s = None -> Empty s.
-     Proof. exact (@M.choose_spec2 _ _). Qed.
-   End Spec.
- End Defs.
- (* TODO: Can this be in a section? *)
- (* Map specs -- require MapsTo to be parameterized by type *)
-  Lemma map_spec1 : forall (A A':Type)(s: t A)(k:key)(e:A)(f:A->A'),
-                      MapsTo k e s -> MapsTo k (f e) (map f s).
-  Proof. exact M.map_spec1. Qed.
-  Lemma map_spec2 : forall (A A':Type)(s: t A)(k:key)(f:A->A'),
-                      In k (map f s) -> In k s.
-  Proof. exact M.map_spec2. Qed.
-  Lemma mapi_spec1 : forall (A A':Type)(m: t A)(x:key)(e:A)(f:key->A->A'), 
-                       MapsTo x e m -> exists y, E.eq y x /\ MapsTo x (f y e) (mapi f m).
-  Proof. exact M.mapi_spec1. Qed.
-  Lemma mapi_spec2 : forall (A A':Type)(m: t A)(x:key)
-                            (f:key->A->A'), In x (mapi f m) -> In x m.
-  Proof. exact M.mapi_spec2. Qed.
-  Lemma map2_spec1 : forall (A A' A'':Type)(m: t A)(m': t A')
-	                        (x:key)(f:option A->option A'->option A''),
-	                   In x m \/ In x m' ->
-                       find x (map2 f m m') = f (find x m) (find x m').
-  Proof. exact M.map2_spec1. Qed.
-  Lemma map2_spec2 : forall (A A' A'':Type)(m: t A)(m': t A')
-	                        (x:key)(f:option A->option A'->option A''),
-                       In x (map2 f m m') -> In x m \/ In x m'.
-  Proof. exact M.map2_spec2. Qed.
+  Lemma MapsTo_spec : E.eq k k' -> MapsTo k v s -> MapsTo k' v s.
+    Admitted.
+
+  Lemma unique: MapsTo k v s -> MapsTo k v' s -> v = v'.
+    Admitted.
+
+  Lemma find_spec : find k s = Some v <-> MapsTo k v s.
+  Admitted.
+
+  Lemma mem_spec : mem k s = true <-> In k s.
+  Proof. exact (@M.mem_spec _ _ _ _). Qed.
+  Lemma equal_1 : Equivb cmp s s' -> equal cmp s s' = true.
+  Proof. exact (@M.equal_1 _ _ _ _ _ _). Qed.
+  Lemma equal_2 : equal cmp s s' = true -> Equivb cmp s s'.
+  Proof. exact (@M.equal_2 _ _ _ _ _ _). Qed.
+  (*
+  Lemma subset_spec : subset s s' = true <-> Subset s s'.
+  Proof. exact (@M.subset_spec _ _ _ _). Qed.
+  *)
+  Lemma empty_spec : Empty empty.
+  Proof. exact (@M.empty_spec _). Qed.
+  Lemma is_empty_spec : is_empty s = true <-> Empty s.
+  Proof. exact (@M.is_empty_spec _ _). Qed.
+  Lemma add_spec1 : E.eq k k' -> MapsTo k v (add k' v s).
+  Proof. exact (@M.add_spec1 _ _ _ _ _ _). Qed.
+  Lemma add_spec2 : ~ E.eq k k' -> (MapsTo k v (add k' v' s) <-> MapsTo k v s).
+  Proof. exact (@M.add_spec2 _ _ _ _ _ _ _). Qed.
+
+  Lemma remove_spec1:  E.eq k k' -> ~ In k (remove k' s).
+  Proof. exact (@M.remove_spec1 _ _ _ _ _). Qed.
+  Lemma remove_spec2: ~ E.eq k k' -> MapsTo k' v (remove k s) <-> MapsTo k' v s.
+  Proof. exact (@M.remove_spec2 _ _ _ _ _ _). Qed.
+  Lemma singleton_spec : E.eq k k' <-> MapsTo k v (singleton k' v).
+  Proof. exact (@M.singleton_spec _ _ _ _). Qed.
+  (*
+  Lemma union_spec : In x (union s s') <-> In x s \/ In x s'.
+  Proof. exact (@M.union_spec _ _ _ _ _). Qed.
+  Lemma inter_spec : In x (inter s s') <-> In x s /\ In x s'.
+  Proof. exact (@M.inter_spec _ _ _ _ _). Qed.
+  Lemma diff_spec : In x (diff s s') <-> In x s /\ ~In x s'.
+  Proof. exact (@M.diff_spec _ _ _ _ _). Qed.
+  *)
+  Lemma fold_spec : forall (X : Type) (i : X) (f : key -> A -> X -> X),
+      fold f s i =
+       fold_left (fun (x : X) (p : key * A) => f (fst p) (snd p) x) (elements s) i.
+  Proof. exact (@M.fold_spec _ _). Qed.
+  Lemma cardinal_spec : cardinal s = length (elements s).
+  Proof. exact (@M.cardinal_spec _ s _). Qed.
+  Lemma filter_spec : compatb f ->
+    (MapsTo k v (filter f s) <-> MapsTo k v s /\ f k v = true).
+  Proof. exact (@M.filter_spec _ _ _ _  _). Qed.
+  Lemma for_all_spec : compatb f ->
+    (for_all f s = true <-> For_all (fun (x : key) (a : A) => f x a = true) s).
+  Proof. exact (@M.for_all_spec _ _ _). Qed.
+  Lemma exists_spec : compatb f ->
+    (exists_ f s = true <-> Exists (fun x a => f x a = true) s).
+  Proof. exact (@M.exists_spec _ _ _). Qed.
+  Lemma partition_spec1 : compatb f -> Equal (fst (partition f s)) (filter f s).
+  Proof. exact (@M.partition_spec1 _ _ _). Qed.
+  Lemma partition_spec2 : compatb f ->
+      Equal (snd (partition f s)) (filter (fun x a => negb (f x a)) s).
+  Proof. exact (@M.partition_spec2 _ _ _). Qed.
+  Lemma elements_spec1 :
+    InA eq_key_elt (k, v) (elements s) <-> MapsTo k v s.
+  Proof. exact (@M.elements_spec1 _ _ _ _). Qed.
+  Lemma elements_spec2w : NoDupA eq_key (elements s).
+  Proof. exact (@M.elements_spec2w _ _). Qed.
+  Lemma choose_spec1 : choose s = Some (k,v) -> MapsTo k v s.
+  Proof. exact (@M.choose_spec1 _ _ _ _). Qed.
+  Lemma choose_spec2 : choose s = None -> Empty s.
+  Proof. exact (@M.choose_spec2 _ _). Qed.
+
+ End Spec.
+ End Foo.
+
 End WRaw2MapsOn.
 
 Module WRaw2Maps (D:DecidableType)(M:WRawMaps D) <: WMaps with Module E := D.
@@ -785,6 +685,8 @@ End WRaw2Maps.
 
 (** Same approach for ordered sets *)
 Module Type RawMaps (E : OrderedType).
+  (* TODO: We have no coparison on maps *)
+  (* Include WRawMaps E <+ HasOrdOps <+ HasLt <+ IsStrOrder. *)
   Include WRawMaps E <+ HasOrdOps.
 
   Section Spec.
@@ -793,12 +695,10 @@ Module Type RawMaps (E : OrderedType).
   Variable k k' : key.
   Variable v v' : A.
 
-  Parameter lt: t A -> t A -> Prop.
-  Global Declare Instance lt_strorder : StrictOrder lt.
-  Global Declare Instance lt_compat : Proper (Logic.eq==>Logic.eq==>iff) lt.
-  
+  (*
   (** Specification of [compare] *)
-  Parameter compare_spec : forall `{Ok _ m, Ok _ m'}, CompSpec Logic.eq lt m m' (compare m m').
+  Parameter compare_spec : forall `{Ok s, Ok s'}, CompSpec eq lt s s' (compare s s').
+  *)
 
   (** Additional specification of [elements] *)
   Parameter elements_spec2 : forall `{Ok _ m}, 
@@ -829,66 +729,66 @@ Module Raw2MapsOn (O:OrderedType)(M:RawMaps O) <: MapsOn O.
   Include WRaw2MapsOn O M.
 
   (* TODO: We have no compare function *)
-  Definition compare {A : Type} (m m':t A) := M.compare m m'.
+  (* Definition compare {A : Type} (m m':t A) := M.compare m m'. *)
   Definition min_elt {A : Type} (m:t A) : option (key * A) := M.min_elt m.
   Definition max_elt {A : Type} (m:t A) : option (key * A) := M.max_elt m.
-  Definition lt {A : Type} (s s':t A) := M.lt s s'.
+  (* Definition lt {A : Type} (s s':t A) := M.lt s s'. *)
+
+  (*
+  (** Specification of [lt] *)
+  Instance lt_strorder : StrictOrder lt.
+  Proof. constructor ; unfold lt; red.
+    unfold complement. red. intros. apply (irreflexivity H).
+    intros. transitivity y; auto.
+  Qed.
+  *)
+
+  (*
+  Instance lt_compat : Proper (eq==>eq==>iff) lt.
+  Proof.
+  repeat red. unfold eq, lt.
+  intros (s1,p1) (s2,p2) E (s1',p1') (s2',p2') E'; simpl.
+  change (M.eq s1 s2) in E.
+  change (M.eq s1' s2') in E'.
+  rewrite E,E'; intuition.
+  Qed.
+  *)
 
   Section Spec.
-    Variable A : Type.
-    Variable m m' m'' : t A.
-    Variable k k' : key.
-    Variable v v' : A.
+  Variable A : Type.
+  Variable m m' m'' : t A.
+  Variable k k' : key.
+  Variable v v' : A.
 
-    (** Specification of [lt] *)
-    Instance lt_strorder : StrictOrder (@lt A).
-    Proof. constructor ; unfold lt; red.
-           unfold complement. red. intros. apply (irreflexivity H).
-           intros. transitivity y; auto.
-    Qed.
+  (*
+  Lemma compare_spec : CompSpec eq lt s s' (compare s s').
+  Proof. unfold compare; destruct (@M.compare_spec s s' _ _); auto. Qed.
+  *)
 
-    Instance lt_compat : Proper (Logic.eq==>Logic.eq==>iff) (@lt A).
-    Admitted.
-    (*
-    Proof.
-      repeat red. unfold eq, lt.
-      intros (s1,p1) (s2,p2) E (s1',p1') (s2',p2') E'; simpl. 
-      change (M.eq s1 s2) in E.
-      change (M.eq s1' s2') in E'.
-      rewrite E,E'; intuition.
-    Qed.
-    *)
+  (** Additional specification of [elements] *)
+  Lemma elements_spec2 : sort (fun p1 p2 => O.lt (fst p1) (fst p2)) (elements m).
+  Proof. exact (@M.elements_spec2 _ _ _). Qed.
 
-    Lemma compare_spec : CompSpec Logic.eq lt m m' (compare m m').
-    Admitted.
-    (*
-    Proof. unfold compare; destruct (@M.compare_spec A m m' _ _); auto. Qed.
-     *)
+  (** Specification of [min_elt] *)
+  Lemma min_elt_spec1 : min_elt m = Some (k, v) -> MapsTo k v m.
+  Proof. exact (@M.min_elt_spec1 _ _ _ _). Qed.
+  Lemma min_elt_spec2 : min_elt m = Some (k, v) -> MapsTo k' v' m -> ~ O.lt k' k.
+  Proof. exact (@M.min_elt_spec2 _ _ _ _ _ _ _). Qed.
+  Lemma min_elt_spec3 : min_elt m = None -> Empty m.
+  Proof. exact (@M.min_elt_spec3 _ _). Qed.
 
-    (** Additional specification of [elements] *)
-    Lemma elements_spec2 : sort (fun p1 p2 => O.lt (fst p1) (fst p2)) (elements m).
-    Proof. exact (@M.elements_spec2 _ _ _). Qed.
+  (** Specification of [max_elt] *)
+  Lemma max_elt_spec1 : max_elt m = Some (k, v) -> MapsTo k v m.
+  Proof. exact (@M.max_elt_spec1 _ _ _ _). Qed.
+  Lemma max_elt_spec2 : max_elt m = Some (k, v) -> MapsTo k' v' m -> ~ O.lt k k'.
+  Proof. exact (@M.max_elt_spec2 _ _ _ _ _ _ _). Qed.
+  Lemma max_elt_spec3 : max_elt m = None -> Empty m.
+  Proof. exact (@M.max_elt_spec3 _ _). Qed.
 
-    (** Specification of [min_elt] *)
-    Lemma min_elt_spec1 : min_elt m = Some (k, v) -> MapsTo k v m.
-    Proof. exact (@M.min_elt_spec1 _ _ _ _). Qed.
-    Lemma min_elt_spec2 : min_elt m = Some (k, v) -> MapsTo k' v' m -> ~ O.lt k' k.
-    Proof. exact (@M.min_elt_spec2 _ _ _ _ _ _ _). Qed.
-    Lemma min_elt_spec3 : min_elt m = None -> Empty m.
-    Proof. exact (@M.min_elt_spec3 _ _). Qed.
-
-    (** Specification of [max_elt] *)
-    Lemma max_elt_spec1 : max_elt m = Some (k, v) -> MapsTo k v m.
-    Proof. exact (@M.max_elt_spec1 _ _ _ _). Qed.
-    Lemma max_elt_spec2 : max_elt m = Some (k, v) -> MapsTo k' v' m -> ~ O.lt k k'.
-    Proof. exact (@M.max_elt_spec2 _ _ _ _ _ _ _). Qed.
-    Lemma max_elt_spec3 : max_elt m = None -> Empty m.
-    Proof. exact (@M.max_elt_spec3 _ _). Qed.
-
-    (** Additional specification of [choose] *)
-    Lemma choose_spec3 :
-      choose m = Some (k, v) -> choose m' = Some (k', v') -> Equal m m' -> O.eq k k'.
-    Proof. exact (@M.choose_spec3 _ _ _ _ _ _ _ _ _). Qed.
+  (** Additional specification of [choose] *)
+  Lemma choose_spec3 :
+    choose m = Some (k, v) -> choose m' = Some (k', v') -> Equal m m' -> O.eq k k'.
+  Proof. exact (@M.choose_spec3 _ _ _ _ _ _ _ _ _). Qed.
 
   End Spec.
 
@@ -899,6 +799,7 @@ Module Raw2Maps (O:OrderedType)(M:RawMaps O) <: Maps with Module E := O.
   Include Raw2MapsOn O M.
 End Raw2Maps.
 
+
 (** It is in fact possible to provide an ordering on sets with
     very little information on them (more or less only the [In]
     predicate). This generic build of ordering is in fact not
@@ -906,6 +807,7 @@ End Raw2Maps.
     dedicated to sets-as-sorted-lists, see [MakeListOrdering].
 *)
 
+(*
 Module Type IN (O:OrderedType).
  Parameter Inline t : Type.
  Parameter Inline In : O.t -> t -> Prop.
@@ -913,65 +815,250 @@ Module Type IN (O:OrderedType).
  Definition Equal s s' := forall x, In x s <-> In x s'.
  Definition Empty s := forall x, ~In x s.
 End IN.
+*)
 
-Module MakeSetOrdering (O:OrderedType)(Import M:IN O).
+Module Type MAPSTO (O:OrderedType).
+ Parameter Inline t : Type -> Type.
+ Variable A : Type.
+ Definition key := O.t.
+ Parameter Inline MapsTo : key -> A -> t A -> Prop.
+ Declare Instance MapsTo_compat : Proper (O.eq==>eq==>eq==>iff) MapsTo.
+ Definition Equal t t' := forall k v, MapsTo k v t <-> MapsTo k v t'.
+ Definition Empty t := forall k v, ~MapsTo k v t.
+End MAPSTO.
+
+Module MakeMapOrdering (O:OrderedType)(Import M:MAPSTO O).
  Module Import MO := OrderedTypeFacts O.
 
- Definition eq : t -> t -> Prop := Equal.
+ Definition eq : t A -> t A -> Prop :=
+ Equal.
 
  Instance eq_equiv : Equivalence eq.
- Proof. firstorder. Qed.
-
- Instance : Proper (O.eq==>eq==>iff) In.
+ Proof. (*firstorder. Qed.*)
+   constructor; try firstorder.
+   constructor.
+   - intros. unfold eq, Equal in *.
+     apply H0. apply H. apply H1.
+   - intros. unfold eq, Equal in *.
+     apply H. apply H0. apply H1.
+ Qed.
+ 
+ Instance : Proper (O.eq==>Logic.eq==>Logic.eq==>iff) MapsTo.
  Proof.
- intros x x' Ex s s' Es. rewrite Ex. apply Es.
+ intros x x' Ex s s' Es.
+ rewrite Ex. rewrite Es. reflexivity.
  Qed.
 
- Definition Below x s := forall y, In y s -> O.lt y x.
- Definition Above x s := forall y, In y s -> O.lt x y.
+ (* am I quantifying v correctly? *)
+ Definition Below k t := forall k' v, MapsTo k' v t -> O.lt k' k.
+ Definition Above k t := forall k' v, MapsTo k' v t -> O.lt k k'.
 
- Definition EquivBefore x s s' :=
-   forall y, O.lt y x -> (In y s <-> In y s').
+ Definition EquivBefore k t t' :=
+   forall k' v, O.lt k' k -> (MapsTo k' v t <-> MapsTo k' v t').
 
- Definition EmptyBetween x y s :=
-   forall z, In z s -> O.lt z y -> O.lt z x.
+ Definition EmptyBetween k1 k2 t :=
+   forall k3 v, MapsTo k3 v t -> O.lt k3 k2 -> O.lt k3 k1.
 
- Definition lt s s' := exists x, EquivBefore x s s' /\
+ Definition lt t t' := exists k, exists v, EquivBefore k t t' /\
+  ((MapsTo k v t' /\ Below k t) \/
+   (MapsTo k v t  /\ exists k' v', MapsTo k' v' t' /\ O.lt k k' /\ EmptyBetween k k' t')).
+
+ (* keeping this around just to be sure... *)
+ (*Definition lt s s' := exists x, EquivBefore x s s' /\
    ((In x s' /\ Below x s) \/
-    (In x s  /\ exists y, In y s' /\ O.lt x y /\ EmptyBetween x y s')).
+    (In x s  /\ exists y, In y s' /\ O.lt x y /\ EmptyBetween x y s')).*)
 
- Instance : Proper (O.eq==>eq==>eq==>iff) EquivBefore.
+ Instance : Proper (O.eq==>Logic.eq==>Logic.eq==>iff) EquivBefore.
  Proof.
   unfold EquivBefore. intros x x' E s1 s1' E1 s2 s2' E2.
   setoid_rewrite E; setoid_rewrite E1; setoid_rewrite E2; intuition.
  Qed.
 
- Instance : Proper (O.eq==>eq==>iff) Below.
+ Instance : Proper (O.eq==>Logic.eq==>iff) Below.
  Proof.
   unfold Below. intros x x' Ex s s' Es.
   setoid_rewrite Ex; setoid_rewrite Es; intuition.
  Qed.
 
- Instance : Proper (O.eq==>eq==>iff) Above.
+ Instance : Proper (O.eq==>Logic.eq==>iff) Above.
  Proof.
   unfold Above. intros x x' Ex s s' Es.
   setoid_rewrite Ex; setoid_rewrite Es; intuition.
  Qed.
 
- Instance : Proper (O.eq==>O.eq==>eq==>iff) EmptyBetween.
+ Instance : Proper (O.eq==>O.eq==>Logic.eq==>iff) EmptyBetween.
  Proof.
   unfold EmptyBetween. intros x x' Ex y y' Ey s s' Es.
   setoid_rewrite Ex; setoid_rewrite Ey; setoid_rewrite Es; intuition.
  Qed.
 
- Instance lt_compat : Proper (eq==>eq==>iff) lt.
+ Instance lt_compat : Proper (Logic.eq==>Logic.eq==>iff) lt.
  Proof.
   unfold lt. intros s1 s1' E1 s2 s2' E2.
   setoid_rewrite E1; setoid_rewrite E2; intuition.
  Qed.
 
+ Ltac isc H := inversion H; subst; clear H.
+
  Instance lt_strorder : StrictOrder lt.
  Proof.
+  pose O.lt_strorder as oltsr.
+  inversion oltsr.
+  unfold Transitive, Irreflexive in *.
+  split.
+  - (* irreflexive *)
+    unfold Irreflexive, Reflexive, complement.
+    intros.
+    isc H. isc H0. isc H. isc H1.
+    +
+      isc H.
+      unfold Below in H2.
+      specialize (H2 x0 x1).
+      apply H2 in H1.
+      apply lt_irrefl in H1.
+      assumption.
+    +
+      isc H. isc H2. isc H. isc H2. isc H3.
+      unfold EmptyBetween in H4.
+      specialize (H4 x0 x1).
+      apply H4 in H1.
+      apply lt_irrefl in H1.
+      assumption.
+      assumption.
+Admitted.
+(* original proof follows. *)
+(*  intros t1 t2 t3 (k & v & EQ & [(MAP2,Pre)|(MAP2,Lex)])
+                  (k' & v' & EQ' & [(MAP2',Pre')|(MAP2',Lex')]).
+  (*intros s1 s2 s3 (x & EQ & [(IN,Pre)|(IN,Lex)])
+                  (x' & EQ' & [(IN',Pre')|(IN',Lex')]).*)
+  (* 1) Pre / Pre --> Pre *)
+  Print Below.
+  assert (O.lt k k').
+  specialize (Pre' k v). apply Pre'; assumption.
+  exists k; exists v; split.
+  unfold EquivBefore. intros k'' v'' Hkk''.
+  rewrite <- (EQ' k'' v''). auto.
+  unfold EquivBefore in EQ'.
+    eapply StrictOrder_Transitive.
+  apply
+  intros y Hy; rewrite <- (EQ' y); auto; order.
+  left; split; auto.
+  rewrite <- (EQ' x); auto.
+  (* 2) Pre / Lex *)
+  elim_compare x x'.
+  (* 2a) x=x' --> Pre *)
+  destruct Lex' as (y & INy & LT & Be).
+  exists y; split.
+  intros z Hz. split; intros INz.
+   specialize (Pre z INz). rewrite <- (EQ' z), <- (EQ z); auto; order.
+   specialize (Be z INz Hz). rewrite (EQ z), (EQ' z); auto; order.
+  left; split; auto.
+  intros z Hz. transitivity x; auto; order.
+  (* 2b) x<x' --> Pre *)
+  exists x; split.
+  intros z Hz. rewrite <- (EQ' z) by order; auto.
+  left; split; auto.
+  rewrite <- (EQ' x); auto.
+  (* 2c) x>x' --> Lex *)
+  exists x'; split.
+  intros z Hz. rewrite (EQ z) by order; auto.
+  right; split; auto.
+  rewrite (EQ x'); auto.
+  (* 3) Lex / Pre --> Lex *)
+  destruct Lex as (y & INy & LT & Be).
+  specialize (Pre' y INy).
+  exists x; split.
+  intros z Hz. rewrite <- (EQ' z) by order; auto.
+  right; split; auto.
+  exists y; repeat split; auto.
+  rewrite <- (EQ' y); auto.
+  intros z Hz LTz; apply Be; auto. rewrite (EQ' z); auto; order.
+  (* 4) Lex / Lex *)
+  elim_compare x x'.
+  (* 4a) x=x' --> impossible *)
+  destruct Lex as (y & INy & LT & Be).
+  setoid_replace x with x' in LT; auto.
+  specialize (Be x' IN' LT); order.
+  (* 4b) x<x' --> Lex *)
+  exists x; split.
+  intros z Hz. rewrite <- (EQ' z) by order; auto.
+  right; split; auto.
+  destruct Lex as (y & INy & LT & Be).
+  elim_compare y x'.
+   (* 4ba *)
+   destruct Lex' as (y' & Iny' & LT' & Be').
+   exists y'; repeat split; auto. order.
+   intros z Hz LTz. specialize (Be' z Hz LTz).
+    rewrite <- (EQ' z) in Hz by order.
+    apply Be; auto. order.
+   (* 4bb *)
+   exists y; repeat split; auto.
+   rewrite <- (EQ' y); auto.
+   intros z Hz LTz. apply Be; auto. rewrite (EQ' z); auto; order.
+   (* 4bc*)
+   assert (O.lt x' x) by auto. order.
+  (* 4c) x>x' --> Lex *)
+  exists x'; split.
+  intros z Hz. rewrite (EQ z) by order; auto.
+  right; split; auto.
+  rewrite (EQ x'); auto.
+ Qed.
+
+
+
+  intros s1 s2 s3 (x & EQ & [(IN,Pre)|(IN,Lex)])
+                  (x' & EQ' & [(IN',Pre')|(IN',Lex')]).
+
+
+    intros t1 t2 t3 (x & EQ & a & b & c).
+
+EQ & [(MAPSTO,Pre)|(MAPSTO,Lex)])
+                  (x' & EQ' & [(IN',Pre')|(IN',Lex')]).
+  
+(* transitive *)
+    unfold Transitive.
+    intros.
+    unfold lt in *.
+    isc H. isc H0. isc H1. isc H. isc H0. isc H1.
+    isc H2; isc H3; isc H1; isc H2.
+    +
+      eexists; eexists.
+      split.
+      unfold EquivBefore in *.
+      unfold Below in *.
+      intros. unfold iff.
+      split. intro.
+      
+
+      apply H4 in H6.      
+      eapply StrictOrder_Transitive in H6.
+      eapply H0 in H2.
+      apply H2.
+      apply H.
+      inversion H2.
+      apply H0.
+      apply H2.
+      apply H.
+      eapply H0 in H2.
+      inversion H2.
+      apply H4 in H6.
+      Print Below.
+      eapply StrictOrder_Transitive.
+      
+      inversion oltsr.
+      unfold StrictOrder, Transitive in s.
+      Print Transitive.
+      Print StrictOrder.
+      SearchAbout O.lt.
+      
+
+      SearchAbout EquivBefore.
+    
+
+ SearchAbout O.lt.
+      Print EmptyBetween.
+      
+  (* original proof *)
   split.
   (* irreflexive *)
   intros s (x & _ & [(IN,Em)|(IN & y & IN' & LT & Be)]).
@@ -1045,71 +1132,78 @@ Module MakeSetOrdering (O:OrderedType)(Import M:IN O).
   right; split; auto.
   rewrite (EQ x'); auto.
  Qed.
+*)
 
  Lemma lt_empty_r : forall s s', Empty s' -> ~ lt s s'.
  Proof.
-  intros s s' Hs' (x & _ & [(IN,_)|(_ & y & IN & _)]).
-  elim (Hs' x IN).
-  elim (Hs' y IN).
- Qed.
+  intros t t' Hs'.
+  intros (k & v & _ & [(M2&_)|(_ & k' & v' & M2 & _)]).
+  elim (Hs' k v M2).
+  elim (Hs' k' v' M2).
+Qed.
 
- Definition Add x s s' := forall y, In y s' <-> O.eq x y \/ In y s.
+ Definition Add k t t' := forall k' v, MapsTo k' v t' <-> O.eq k k' \/ MapsTo k' v t.
 
- Lemma lt_empty_l : forall x s1 s2 s2',
-  Empty s1 -> Above x s2 -> Add x s2 s2' -> lt s1 s2'.
+ Lemma lt_empty_l : forall k (v : A) t1 t2 t2',
+  Empty t1 -> Above k t2 -> Add k t2 t2' -> lt t1 t2'.
  Proof.
-  intros x s1 s2 s2' Em Ab Ad.
-  exists x; split.
-  intros y Hy; split; intros IN.
-  elim (Em y IN).
-  rewrite (Ad y) in IN; destruct IN as [EQ|IN]. order.
-  specialize (Ab y IN). order.
+  intros k v t1 t2 t2' Em Ab Ad.
+  exists k. exists v. split.
+  intros k' v' Hk'. split; intros M2.
+  elim (Em k' v' M2).
+  rewrite (Ad k') in M2. destruct M2 as [EQ|M2]. order.
+  specialize (Ab k' v' M2). order.
   left; split.
-  rewrite (Ad x). now left.
-  intros y Hy. elim (Em y Hy).
+  rewrite (Ad k). now left.
+  intros k' v' Hk'. elim (Em k' v' Hk').
  Qed.
 
- Lemma lt_add_lt : forall x1 x2 s1 s1' s2 s2',
-   Above x1 s1 -> Above x2 s2 -> Add x1 s1 s1' -> Add x2 s2 s2' ->
-   O.lt x1 x2 -> lt s1' s2'.
+ Lemma lt_add_lt : forall k1 k2 (v : A) t1 t1' t2 t2',
+   Above k1 t1 -> Above k2 t2 -> Add k1 t1 t1' -> Add k2 t2 t2' ->
+   O.lt k1 k2 -> lt t1' t2'.
   Proof.
-  intros x1 x2 s1 s1' s2 s2' Ab1 Ab2 Ad1 Ad2 LT.
-  exists x1; split; [ | right; split]; auto.
-  intros y Hy. rewrite (Ad1 y), (Ad2 y).
+  intros k1 k2 v t1 t1' t2 t2' Ab1 Ab2 Ad1 Ad2 LT.
+  exists k1; exists v; split; [ | right; split]; auto.
+  intros k' v' Hk'. rewrite (Ad1 k'), (Ad2 k').
   split; intros [U|U]; try order.
-  specialize (Ab1 y U). order.
-  specialize (Ab2 y U). order.
-  rewrite (Ad1 x1); auto with *.
-  exists x2; repeat split; auto.
-  rewrite (Ad2 x2); now left.
-  intros y. rewrite (Ad2 y). intros [U|U]. order.
-  specialize (Ab2 y U). order.
+  specialize (Ab1 k' v' U). order.
+  specialize (Ab2 k' v' U). order.
+  rewrite (Ad1 k1); auto with *.
+  exists k2; exists v; repeat split; auto.
+  rewrite (Ad2 k2 v); now left.
+  intros k' v'. rewrite (Ad2 k' v'). intros [U|U]. order.
+  specialize (Ab2 k' v' U). order.
   Qed.
 
-  Lemma lt_add_eq : forall x1 x2 s1 s1' s2 s2',
-   Above x1 s1 -> Above x2 s2 -> Add x1 s1 s1' -> Add x2 s2 s2' ->
-   O.eq x1 x2 -> lt s1 s2 -> lt s1' s2'.
+  Lemma lt_add_eq : forall k1 k2 (v : A) t1 t1' t2 t2',
+   Above k1 t1 -> Above k2 t2 -> Add k1 t1 t1' -> Add k2 t2 t2' ->
+   O.eq k1 k2 -> lt t1 t2 -> lt t1' t2'.
   Proof.
-  intros x1 x2 s1 s1' s2 s2' Ab1 Ab2 Ad1 Ad2 Hx (x & EQ & Disj).
-  assert (O.lt x1 x).
-   destruct Disj as [(IN,_)|(IN,_)]; auto. rewrite Hx; auto.
-  exists x; split.
-  intros z Hz. rewrite (Ad1 z), (Ad2 z).
+  intros k1 k2 v1 t1 t1' t2 t2' Ab1 Ab2 Ad1 Ad2 Hx (k & v & EQ & Disj).
+  assert (O.lt k1 k).
+   destruct Disj as [(M2,_)|(M2,_)]; auto. rewrite Hx.
+   apply (Ab2 k v). auto.
+   apply (Ab1 k v). auto.
+  exists k; exists v; split.
+  intros k'' v'' Hk''. rewrite (Ad1 k''), (Ad2 k'').
   split; intros [U|U]; try (left; order); right.
-  rewrite <- (EQ z); auto.
-  rewrite (EQ z); auto.
-  destruct Disj as [(IN,Em)|(IN & y & INy & LTy & Be)].
+  rewrite <- (EQ k''); auto.
+  rewrite (EQ k''); auto.
+  destruct Disj as [(M2,Em)|(M2 & k' & v' & M2k' & LTk' & Be)].
   left; split; auto.
-  rewrite (Ad2 x); auto.
-  intros z. rewrite (Ad1 z); intros [U|U]; try specialize (Ab1 z U); auto; order.
+  rewrite (Ad2 k); auto.
+  intros k'' v''.
+  rewrite (Ad1 k''); intros [U|U]; try specialize (Ab1 k'' v'' U). order.
+    unfold Below in Em. apply (Em k'' v''). auto.
   right; split; auto.
-  rewrite (Ad1 x); auto.
-  exists y; repeat split; auto.
-  rewrite (Ad2 y); auto.
-  intros z. rewrite (Ad2 z). intros [U|U]; try specialize (Ab2 z U); auto; order.
+  rewrite (Ad1 k); auto.
+  exists k'; exists v'; repeat split; auto.
+  rewrite (Ad2 k'); auto.
+  intros k'' v''. rewrite (Ad2 k''). intros [U|U]; try specialize (Ab2 k'' v'' U). order.
+    intro H2. unfold EmptyBetween in Be. apply (Be k'' v''); auto.
   Qed.
 
-End MakeSetOrdering.
+End MakeMapOrdering.
 
 
 Module MakeListOrdering (O:OrderedType).
@@ -1188,3 +1282,4 @@ Module MakeListOrdering (O:OrderedType).
 
 End MakeListOrdering.
 
+*)
